\documentclass{article}

\usepackage[margin=2cm]{geometry}
\usepackage{amsmath,amsfonts,graphicx,listings}

\title{Formulation}
\author{}

\date{}

\begin{document}
\maketitle

We can always choose the coordinate system such that the start point is $(0,0)$ and the terminal be $(0,y)$
\section{Notation}
Denote the boundary of the each flow region be $f(x)$, which should be continuous and has corresponding subgradients.
Suppose a path $\gamma$ from $(x_0,f_0(x_0))=(0,0)$ to $(x_n,f_n(x_n))=(0,y)$ intersects the flow region boundaries at $\{(x_i,f_i)\}_{i=0}^n$ where $f_i=f_i(x_i)$ and denote the robot velocity in each region be $v=(v_x^i,v_y^i)$ and the flow velocity be $u=(u_x^i,u_y^i)$. Also the speed of robot has an upper bound, say $V$ (i.e. $(v_x^i)^2+(v_y^i)^2\leq V^2$). And the time used in each region be $t_i$ and the total time consumption is $T(\gamma)=\sum_{i=1}^nt_i(\gamma)$. The problem is $\min_{\gamma} T(\gamma)$\\\\
\textbf{Property} To achieve the optimality, in each region, the robot should move with maximum speed.\\
If not, say in region $i$, $(v_x^i)^2+(v_y^i)^2<V^2$, then we can let the speed be $(v_x^i+\epsilon,v_y^i+\eta)$ such that $(v_y^i-u_y^i)\epsilon=(v_x^i-u_x^i)\eta$. Since $\epsilon$ and $\eta$ can be sufficiently small, the speed can always achieve the upper bound with the moving direction unchanged, which is because
\[
\frac{v_x^i-u_x^i}{v_y^i-u_y^i}=\frac{v_x^i-u_x^i+\epsilon}{v_y^i-u_y^i+\eta}
\]

Thus, we can always rewrite $(v_x^i,v_y^i)=(V\cos\theta_i,V\sin\theta_i)$

\section{Formulation}
The optimization is
\begin{align*}
\min_{x_1,\cdots,x_{n-1}}&\sum_{t=1}^nt_i(x_i)\\\text{s.t.}\ \ &x_0=x_n=0\\&f_n=y
\end{align*}
within which, we take one specific term $t_i$ and ignore the super- and sub-script, that is $t=t_i,v_x=v_x^i,x=x_i,f=f_i=f_i(x_i),x^-=x_{i-1},f^-=f_{i-1}=f_{i-1}(x_{i-1})$ etc. We know that
\begin{align*}
&\frac{x-x^-}{f-f^-}=\frac{v_x-u_x}{v_y-u_y}\\
\Rightarrow&(x-x^-)(V\sin\theta-u_y)=(f-f^-)(V\cos\theta-u_x)\\
\Rightarrow&(f-f^-)\cos\theta-(x-x^-)\sin\theta=\frac{1}{V}(u_x(f-f^-)-u_y(x-x^-))\\
\Rightarrow&\cos(\theta+\alpha)=\frac{u_x(f-f^-)-u_y(x-x^-)}{V\sqrt{(f-f^-)^2+(x-x^-)^2}}
\end{align*}
where
\[
\cos\alpha=\frac{f-f^-}{\sqrt{(f-f^-)^2+(x-x^-)^2}},\sin\alpha=\frac{x-x^-}{\sqrt{(f-f^-)^2+(x-x^-)^2}}
\]
Denote
\begin{align*}
C=\frac{u_x(f-f^-)-u_y(x-x^-)}{V\sqrt{(f-f^-)^2+(x-x^-)^2}}
\end{align*}
Then, $\theta=-\alpha\pm\arccos C$
\begin{align*}
\cos\theta=&\cos(-\alpha\pm\arccos C)=C\cos\alpha\mp\sqrt{1-C^2}\sin\alpha\\
\sin\theta=&\sin(-\alpha\pm\arccos C)=-C\sin\alpha\pm\sqrt{1-C^2}\cos\alpha
\end{align*}
Then back to add the super- and sub-script, we have
\begin{align}
&C_i=\frac{u_x^i(f_i-f_{i-1})-u_y^i(x_i-x_{i-1})}{V\sqrt{(f_i-f_{i-1})^2+(x_i-x_{i-1})^2}}\label{equ:1}\\
&\cos\alpha_i=\frac{f_i-f_{i-1}}{\sqrt{(f_i-f_{i-1})^2+(x_i-x_{i-1})^2}}\label{equ:2}\\
&\sin\alpha_i=\frac{x_i-x_{i-1}}{\sqrt{(f_i-f_{i-1})^2+(x_i-x_{i-1})^2}}\label{equ:3}\\
&\cos\theta_i=\cos(-\alpha_i\pm\arccos C_i)=C_i\cos\alpha_i\mp\sqrt{1-C_i^2}\sin\alpha_i\label{equ:4}\\
&\sin\theta_i=\sin(-\alpha_i\pm\arccos C_i)=-C_i\sin\alpha_i\pm\sqrt{1-C_i^2}\cos\alpha_i\label{equ:5}
\end{align}
Combine (\ref{equ:1})-(\ref{equ:5}), the final optimization is
\begin{align*}
\min_{x_1,\cdots,x_{n-1}}&\sum_{i=1}^n\frac{\sqrt{(x_i-x_{i-1})^2+(f_i-f_{i-1})^2}}{\sqrt{(V\cos\theta_i-u_x^i)^2+(V\sin\theta_i-u_y^i)^2}}\\
\text{s.t.}\ \ &x_0=x_n=0\\&f_n=y
\end{align*}

\end{document}




